Blanc/ReWeth.lean
@@ -1,0 +1,325 @@
+-- Weth.lean : proof-of-concept implementation of the Wrapped Ether (WETH) contract
+
+import Blanc.ReCommon
+
+
+
+open Ninst
+
+-- deposit() --
+
+def logDeposit : Func :=
+  callvalue ::: mstoreAt 0 +++ caller ::: -- caller || wad
+  pushB256 "Deposit(address,uint256)".keccak ::: -- depositEventSig :: caller || wad
+  logWith 1 0 1 +++ -- 1 indexed topic : caller address
+                    -- 1 unindexed data : deposit value
+  Func.stop
+
+def deposit : Func :=
+  caller ::: sload ::: -- caller_bal
+  callvalue ::: add ::: -- (call_val + caller_bal)
+  caller ::: -- caller :: (call_val + caller_bal)
+  sstore ::: -- caller WETH balance is now up to date
+  logDeposit
+
+
+
+-- withdraw(uint wad) --
+
+-- assumes : args := [wad]
+def logWithdraw : Func :=
+  caller :::
+  pushB256 "Withdrawal(address,uint256)".keccak ::: -- withdrawEventSig :: caller
+  argCopy 0 0 1 +++ -- withdrawEventSig :: caller || wad
+  logWith 1 0 1 +++ -- 1 indexed topic : caller address
+                    -- 1 unindexed data : withdraw amount
+  Func.stop
+
+-- ( wad -- )
+def sendToCaller : Line :=
+  pushList [0, 0, 0, 0] ++ -- 0 :: 0 :: 0 :: 0 :: wad
+  swap 3 :: caller :: -- caller :: wad :: 0 :: 0 :: 0 :: 0
+  push [0x52, 0x08] (by {simp [List.length]}) :: -- 21000 :: caller :: wad :: 0 :: 0 :: 0 :: 0
+  call :: -- 'wad' amount of ethers now sent to 'caller'
+  []
+
+-- assumes : args := [wad]
+def withdrawLoadCheck : Line :=
+  arg 0 ++ dup 0 :: -- wad :: wad
+  caller :: sload :: -- caller_bal :: wad :: wad
+  dup 1 :: dup 1 :: -- caller_bal :: wad :: caller_bal :: wad :: wad
+  lt :: -- (caller_bal < wad) :: caller_bal :: wad :: wad
+  []
+
+-- assumes : args := [wad]
+def withdraw : Func :=
+  withdrawLoadCheck +++ -- (caller_bal < wad) :: caller_bal :: wad :: wad
+  .rev <?> -- [if caller balance < withdraw amount, revert]
+           -- caller_bal :: wad :: wad
+  sub ::: caller ::: -- caller :: (caller_bal - wad) :: wad
+  sstore ::: -- wad
+             -- 'wad' amount of eth subtracted from caller balance
+  sendToCaller +++
+  logWithdraw
+
+
+
+-- decimals() --
+
+def decimals : Func :=
+  pushB256 0x12 ::: -- 0x12 ||
+  mstoreAt 0 +++ -- || 0x12
+  returnMemoryRange 0 32
+
+
+
+-- name() --
+
+def name : Func :=
+  --pushB256 wrappedEtherStringShift ::: -- wrappedEtherStringShift ||
+  pushB256 "Wrapped Ether".toB8L.toB256 :::
+  pushB256 152 ::: shl ::: -- "Wrapped Ether" ||
+  pushList [13, 32] +++ -- 32 :: 13 :: "Wrapped Ether" ||
+  mstoreAt 0 +++ -- 13 :: "Wrapped Ether" || 32
+  mstoreAt 1 +++ -- "Wrapped Ether" || 32 13
+  mstoreAt 2 +++ -- || 32 13 "Wrapped Ether"
+  returnMemoryRange 0 96
+
+
+
+-- symbol() --
+
+def symbol : Func :=
+  -- pushList [wethStringShift] +++ -- wethStringShift
+  pushB256 "WETH".toB8L.toB256 :::
+  pushB256 224 ::: shl ::: -- "WETH""
+  pushList [4, 32] +++ -- 32 :: 4 :: "WETH""
+  mstoreAt 0 +++ -- 4 :: "WETH"" || 32
+  mstoreAt 1 +++ -- "WETH" || 32 4
+  mstoreAt 2 +++ -- || 32 4 "WETH""
+  returnMemoryRange 0 96
+
+
+
+-- balanceOf(address guy) --
+
+def balanceOf : Func :=
+  arg 0 +++ -- guy ||
+  sload ::: -- guy_bal ||
+  mstoreAt 0 +++ -- || guy_bal
+  returnMemoryRange 0 32
+
+
+
+-- allowance(address src, address dst) --
+
+def allowance : Func :=
+  argCopy 0 0 2 +++ -- || src dst
+  pushList [64, 0] +++ -- 0 :: 64 || src dst
+  kec ::: -- hash ||
+  sload ::: -- allowAmnt ||
+  mstoreAt 0 +++ -- || allow_amnt
+  returnMemoryRange 0 32
+
+
+
+-- totalSuppply() --
+
+def totalSupply : Func :=
+  address ::: balance ::: -- total_bal ||
+  mstoreAt 0 +++ -- || total_bal
+  returnMemoryRange 0 32
+
+
+
+-- approve(address guy, uint wad) --
+
+-- assumes : args = [guy, wad]
+-- ( -- caller_guy_hash_valid? :: caller_guy_hash :: wad )
+def prepApprove : Line :=
+  caller :: mstoreAt 0 ++ -- || caller
+  argCopy 1 0 1 ++ -- || caller :: guy
+  arg 1 ++ pushList [64, 0] ++ -- 0 :: 64 :: wad || caller :: guy
+  kec :: dup 0 :: -- caller_guy_hash :: caller_guy_hash :: wad ||
+  checkAddress  -- caller_guy_hash_valid? :: caller_guy_hash :: wad ||
+
+-- assumes : args = [guy, wad]
+def logApprove : Line :=
+  argCopy 0 1 1 ++ -- || wad
+  arg 0 ++ caller ::
+  pushB256 "Approval(address,address,uint256)".keccak :: -- approvalEventSig :: caller :: guy || wad
+  logWith 2 0 1 -- 2 indexed topics : caller address, approvee address
+                -- 1 unindexed data : approval value
+
+
+-- arguments = [guy, wad]
+def approve : Func :=
+  arg 0 +++ -- guy ||
+  checkNonAddress +++ -- guy_invalid? ||
+  .rev <?> -- [if guy is invalid, revert]
+  prepApprove +++ -- hash_valid? :: hash :: wad ||
+  .rev <?> -- [ if storage location of approval amount
+           --   is a valid address that may potentially
+           --   collide with balance storage, revert ]
+           -- hash :: wad ||
+  sstore :: -- ||
+  logApprove +++
+  returnTrue
+
+
+
+-- transfer(address dst, uint wad) --
+
+-- assumes : args = [dst, wad]
+def logTransfer : Line :=
+  argCopy 0 1 1 ++ -- || wad
+  arg 0 ++ caller ::
+  pushB256 "Transfer(address,address,uint256)".keccak :: -- transferEventSig :: src :: dst || wad
+  logWith 2 0 1 -- 2 indexed topics : source address, destination address
+                -- 1 unindexed data : transfer value
+
+-- ( wad dst -- )
+def incrWbal : Line :=
+  dup 1 :: -- dst :: wad :: dst
+  sload :: -- dst_bal :: wad :: dst
+  add :: -- (dst_bal + wad) :: dst
+  swap 0 :: -- dst :: (dst_bal + wad)
+  sstore :: []
+
+-- assumes : arg = [dst, wad]
+-- ( -- dst_invalid :: dst )
+def transferTestDst : Line :=
+  arg 0 ++ dup 0 :: -- dst :: dst
+  checkNonAddress -- dst_invalid :: dst
+
+-- assumes : arg = [_, wad]
+-- ( -- caller_bal_<_wad? caller_bal wad wad )
+def transferTestLt : Line :=
+  arg 1 ++ -- wad :: dst
+  caller :: -- caller :: wad :: dst
+  dup 0 :: -- caller :: caller :: wad :: dst
+  sload :: -- caller_bal :: caller :: wad :: dst
+  swap 0 :: -- caller :: caller_bal :: wad :: dst
+  dup 2 :: -- wad :: caller :: caller_bal :: wad :: dst
+  dup 0 :: -- wad :: wad :: caller :: caller_bal :: wad :: dst
+  dup 3 :: -- caller_bal :: wad :: wad :: caller :: caller_bal :: wad :: dst
+  sub ::   -- caller_bal - wad :: wad :: caller :: caller_bal :: wad :: dst
+  swap 2 :: -- caller_bal :: wad :: caller :: caller_bal - wad :: wad :: dst
+  lt :: [] -- caller_bal_<_wad? :: caller :: caller_bal - wad :: wad :: dst
+
+-- ( caller :: caller_bal - wad :: wad :: dst -- * )
+def transferCore : Func :=
+  sstore ::: -- wad :: dst [caller balance up to date]
+  incrWbal +++ -- [destination balance up todate]
+  logTransfer +++
+  returnTrue
+
+-- assumes : arg = [dst, wad]
+def transfer : Func :=
+  transferTestDst +++ -- dst_invalid? :: dst
+  .rev <?> -- [if dst is not a valid address, revert]
+           -- dst
+  transferTestLt +++ -- (caller_bal < wad) :: caller :: caller_bal - wad :: wad :: dst
+  .rev <?> -- [if caller balance < transfer amount, revert]
+        -- caller :: caller_bal - wad :: wad :: dst
+  transferCore
+
+-- ( sbal :: wad :: wad :: src -- wad :: src )
+def transferFromUpdateSbal : Line :=
+  sub :: -- (sbal - wad) :: wad :: src
+  dup 2 :: -- src :: (sbal - wad) :: wad :: src
+  sstore :: -- [source balance is up to date]
+  []        -- wad :: src
+
+-- ( dst :: wad :: src -- wad :: src )
+def transferFromLog : Line :=
+  dup 2 :: -- src :: dst :: wad :: src
+  pushB256 "Transfer(address,address,uint256)".keccak :: -- transferEventSig :: src :: dst :: wad :: src
+  dup 3 :: mstoreAt 0 ++ -- transferEventSig :: src :: dst :: wad :: src || wad
+  logWith 2 0 1 -- [Transfer(src,dst,wad) is logged]
+                -- wad :: src
+
+-- (wad src -- )
+def updateAllowance : Func :=
+  prepend [caller, dup 2, eq] <| -- (src =? caller) :: wad :: src
+  returnTrue <?> -- if caller is source, do not update allowance
+                 -- wad :: src
+  swap 0 :: mstoreAt 0 +++ -- wad || src
+  caller ::: mstoreAt 1 +++ -- wad || src :: caller
+  pushList [64, 0] +++ -- 0 :: 64 :: wad || src :: caller
+  kec ::: -- hash :: wad
+  swap 0 ::: -- wad :: hash
+  dup 1 :: checkAddress +++ -- va(hash) :: wad :: hash
+  .rev <?> -- if hash is a valid address, revert to prevent collision
+           -- wad :: hash
+  dup 1 ::: sload ::: -- amnt :: wad :: hash
+  dup 0 ::: isMax +++ -- (amnt =? max) :: amnt :: wad :: hash
+  returnTrue <?> -- if allowed amount is infinite (per EIP-717), do not update allowance
+                 -- amnt :: wad :: hash
+  dup 1 ::: dup 1 ::: lt ::: -- amnt <? wad :: amnt :: wad :: hash
+  .rev <?> -- if allowed amount < transfer amount, revert
+           -- amnt :: wad :: hash
+  sub ::: swap 0 ::: -- hash :: (amnt - wad)
+  sstore ::: returnTrue -- [allowance amount is up to date]
+
+-- assumes : args = [src, dst, wad]
+def transferFrom : Func :=
+  arg 0 +++ dup 0 ::: checkNonAddress +++ -- ¬ va(src) :: src
+  .rev <?> -- [if src is not a valid address, revert]
+        -- src
+  arg 2 +++ dup 0 ::: dup 2 ::: sload ::: -- sbal :: wad :: wad :: src
+  dup 1 ::: dup 1 ::: lt ::: -- (sbal <? wad) :: sbal :: wad :: wad :: src
+  .rev <?> -- if source balance < wad, then revert
+        -- sbal :: wad :: wad :: src
+  transferFromUpdateSbal +++ -- wad :: src
+  arg 1 +++ dup 0 ::: checkNonAddress +++ -- ¬ va(dst) :: dst :: wad :: src
+  .rev <?> -- [if dst is not a valid address, revert]
+        -- dst :: wad :: src
+  dup 0 ::: dup 2 ::: -- wad :: dst :: dst :: wad :: src
+  incrWbal +++ -- [destination balance is up to date]
+              -- dst :: wad :: src
+  transferFromLog +++ -- wad :: src
+  updateAllowance
+
+
+
+-- main --
+
+inductive ArgType
+  | address
+  | uint256
+
+def ArgType.toString : ArgType → String
+  | address => "address"
+  | uint256 => "uint256"
+
+def selectorArgs : List ArgType → String
+  | [] => ""
+  | t :: ts => List.foldl (λ s t' => s!"{s},{t'.toString}") t.toString ts
+
+def selector (name : String) (args : List ArgType) : B256 :=
+  (s!"{name}({selectorArgs args})").keccak.shiftRight 224
+
+def wethTree : DispatchTree :=
+  .fork
+  ( .fork
+    ( .fork
+      ( .fork
+        (.leaf (selector "name" []) name)
+        (.leaf (selector "approve" [.address, .uint256]) approve) )
+      (.leaf (selector "totalSupply" []) totalSupply)
+    )
+    ( .fork
+      (.leaf (selector "transferFrom" [.address, .address, .uint256]) transferFrom)
+      (.leaf (selector "withdraw" [.uint256]) withdraw) ) )
+  ( .fork
+    ( .fork
+      ( .fork
+        (.leaf (selector "decimals" []) decimals)
+        (.leaf (selector "balanceOf" [.address]) balanceOf) )
+      (.leaf (selector "symbol" []) symbol) )
+    ( .fork
+      (.leaf (selector "transfer" [.address, .uint256]) transfer)
+      (.leaf (selector "allowance" [.address, .address]) allowance) ) )
+
+def weth : Prog := ⟨Func.mainWith 1 wethTree, [deposit]⟩
